switch core from nat to w64

src/program_proof/pav/core.v
@@ -2,8 +2,9 @@ From Perennial.program_proof Require Import grove_prelude.
 From Perennial.program_proof.pav Require Import serde.
 
 From RecordUpdate Require Export RecordSet.
-From Perennial.base_logic.lib Require Export ghost_map.
 From iris.unstable.base_logic Require Export mono_list.
+From Perennial.base_logic.lib Require Export ghost_map.
+From Perennial.Helpers Require Import Integers.
 
 (* TODO: for same reason not using alias's in go code,
 prob shouldn't define all these notations. *)
@@ -11,23 +12,17 @@ Notation comm_ty := (list w8) (only parsing).
 Notation dig_ty := (list w8) (only parsing).
 Notation uid_ty := w64 (only parsing).
 Notation ver_ty := w64 (only parsing).
-(* TODO: make fake_ver_ty, fake_epoch_ty work for w64. *)
-Notation fake_ver_ty := nat (only parsing).
 Notation epoch_ty := w64 (only parsing).
-Notation fake_epoch_ty := nat (only parsing).
 Notation pk_ty := (list w8) (only parsing).
 Notation map_label_ty := (uid_ty * ver_ty)%type (only parsing).
-Notation fake_map_label_ty := (uid_ty * fake_ver_ty)%type (only parsing).
 Notation opaque_label_ty := (list w8) (only parsing).
 Notation map_val_ty := (epoch_ty * pk_ty)%type (only parsing).
-Notation fake_map_val_ty := (fake_epoch_ty * pk_ty)%type (only parsing).
 Notation map_ty := (gmap map_label_ty map_val_ty) (only parsing).
-Notation fake_map_ty := (gmap fake_map_label_ty fake_map_val_ty) (only parsing).
 Notation merkle_map_ty := (gmap (list w8) (list w8)) (only parsing).
 Notation map_adtr_ty := (gmap opaque_label_ty (epoch_ty * comm_ty)) (only parsing).
 Notation cli_map_val_ty := (option (epoch_ty * comm_ty))%type (only parsing).
 Notation cli_map_ty := (gmap map_label_ty cli_map_val_ty) (only parsing).
-Notation lat_val_ty := (option (fake_ver_ty * fake_map_val_ty)) (only parsing).
+Notation lat_val_ty := (option (ver_ty * map_val_ty)) (only parsing).
 
 Section misc.
 Class pavG Σ :=
@@ -42,12 +37,13 @@ Section msv_core.
 
 (* maximum sequence of versions. *)
 
-Definition msv_core_aux (m : fake_map_ty) uid (vals : list fake_map_val_ty) :=
-  (∀ ver val, vals !! ver = Some val → m !! (uid, ver) = Some val).
+Definition msv_core_aux (m : map_ty) uid (vals : list map_val_ty) :=
+  length vals < 2^64 ∧
+  (∀ (ver : w64) val, vals !! (uint.nat ver) = Some val → m !! (uid, ver) = Some val).
 
 Definition msv_core m uid vals :=
   msv_core_aux m uid vals ∧
-  m !! (uid, (length vals)) = None.
+  m !! (uid, W64 (length vals)) = None.
 
 (* TODO: upstream. *)
 Lemma lookup_snoc {A} (l : list A) (x : A) :
@@ -56,12 +52,13 @@ Proof. by opose proof (proj2 (lookup_snoc_Some x l (length l) x) _) as H; [naive
 
 Lemma msv_core_aux_snoc {m uid l x} :
   msv_core_aux m uid (l ++ [x]) →
-  msv_core_aux m uid l ∧ m !! (uid, length l) = Some x.
+  msv_core_aux m uid l ∧ m !! (uid, W64 (length l)) = Some x.
 Proof.
-  intros HM. split.
-  - intros ?? Hlook. ospecialize (HM _ _ _); [|done].
+  intros [Hlen HM]. rewrite app_length in Hlen. list_simplifier. split.
+  - split; [lia|]. intros ?? Hlook. ospecialize (HM _ _ _); [|done].
     rewrite lookup_app_l; [exact Hlook|by eapply lookup_lt_Some].
-  - ospecialize (HM (length l) _ _); [apply lookup_snoc|done].
+  - ospecialize (HM (length l) _ _); [|done].
+    rewrite nat_thru_w64_id; [|lia]. apply lookup_snoc.
 Qed.
 
 Lemma msv_core_aux_agree {m uid vals0 vals1} :
@@ -87,8 +84,8 @@ Lemma msv_core_len_agree_aux {m uid vals0 vals1} :
   length vals0 < length vals1 →
   False.
 Proof.
-  intros HM0 HM1 ?. destruct HM0 as [_ HM0], HM1 as [HM1 _].
-  list_elem vals1 (length vals0) as val.
+  intros HM0 HM1 ?. destruct HM0 as [_ HM0], HM1 as [[? HM1] _].
+  list_elem vals1 (uint.nat (length vals0)) as val.
   ospecialize (HM1 _ _ _); [exact Hval_lookup|naive_solver].
 Qed.
 
@@ -121,8 +118,8 @@ Section msv.
 
 (* msv hides all but the latest val.
 a None val corresponds to an unregistered val. *)
-Definition msv (m : fake_map_ty) uid (lat : lat_val_ty) :=
-  let len_vals := match lat with None => 0 | Some (ver, val) => S ver end in
+Definition msv (m : map_ty) uid (lat : lat_val_ty) :=
+  let len_vals := match lat with None => 0%nat | Some (ver, val) => S (uint.nat ver) end in
   ∃ vals, length vals = len_vals ∧ last vals = snd <$> lat ∧
   msv_core m uid vals.
 
@@ -134,7 +131,8 @@ Proof.
   intros HM0 HM1.
   destruct HM0 as (?&Hlen0&?&HM0). destruct HM1 as (?&Hlen1&?&HM1).
   pose proof (msv_core_agree HM0 HM1) as ->. rewrite Hlen0 in Hlen1.
-  destruct val0 as [[??]|], val1 as [[??]|]; naive_solver.
+  destruct val0 as [[ver0 ?]|], val1 as [[ver1 ?]|]; [|done..].
+  assert (ver0 = ver1) as -> by word. naive_solver.
 Qed.
 
 End msv.
@@ -144,52 +142,55 @@ Section hist_msv.
 (* history and its interaction with msv. *)
 
 (* for now, duplicate adtr invs so that below proofs can use this more pure version. *)
-Definition maps_mono' (ms : list fake_map_ty) :=
-  ∀ i j mi mj,
-  ms !! i = Some mi →
-  ms !! j = Some mj →
-  i ≤ j →
+Definition maps_mono' (ms : list map_ty) :=
+  ∀ (i j : w64) mi mj,
+  ms !! uint.nat i = Some mi →
+  ms !! uint.nat j = Some mj →
+  uint.Z i ≤ uint.Z j →
   mi ⊆ mj.
 
 (* maps_epoch_ok prevents entries from being added too early. *)
-Definition maps_epoch_ok' (ms : list fake_map_ty) :=
-  ∀ ep m k ep' comm,
-  ms !! ep = Some m →
+Definition maps_epoch_ok' (ms : list map_ty) :=
+  ∀ (ep : w64) m k ep' comm,
+  ms !! (uint.nat ep) = Some m →
   m !! k = Some (ep', comm) →
-  ep' ≤ ep.
+  uint.Z ep' ≤ uint.Z ep.
 
 Definition adtr_inv' ms := maps_mono' ms ∧ maps_epoch_ok' ms.
 
 (* TODO: this is one way to write it. consolidates cases.
 let's see how easy it is to prove with the physical hist. *)
-Definition know_hist_val (ms : list fake_map_ty) (uid : w64) (ep : nat) (lat : lat_val_ty) :=
-  let len_vals := match lat with None => 0 | Some (ver, val) => S ver end in
-  ∃ vals, length vals = len_vals ∧ last vals = snd <$> lat ∧
+Definition know_hist_val (ms : list map_ty) (uid : w64) (ep : w64) (lat : lat_val_ty) :=
+  let len_vals := match lat with None => 0%nat | Some (ver, val) => S (uint.nat ver) end in
+  ∃ vals, length vals = len_vals ∧ length vals < 2^64 ∧ last vals = snd <$> lat ∧
   (* prior vers exist in prior or this map. *)
-  (∀ ver val, vals !! ver = Some val →
-    (∃ prior m, prior ≤ ep ∧ ms !! prior = Some m ∧ m !! (uid, ver) = Some val)) ∧
+  (∀ (ver : w64) val, vals !! uint.nat ver = Some val →
+    (∃ (prior : w64) m, uint.Z prior ≤ uint.Z ep ∧ ms !! uint.nat prior = Some m ∧
+      m !! (uid, ver) = Some val)) ∧
   ( (* next ver doesn't exist in this or later map. *)
-    (∃ bound m, bound ≥ ep ∧ ms !! bound = Some m ∧ m !! (uid, length vals) = None)
+    (∃ (bound : w64) m, uint.Z ep ≤ uint.Z bound ∧ ms !! uint.nat bound = Some m ∧
+      m !! (uid, W64 (length vals)) = None)
     ∨
     (* next ver exists in later map. *)
-    (∃ bound m comm, bound > ep ∧ ms !! bound = Some m ∧ m !! (uid, length vals) = Some (bound, comm))).
+    (∃ (bound : w64) m comm, uint.Z ep < uint.Z bound ∧ ms !! uint.nat bound = Some m ∧
+      m !! (uid, W64 (length vals)) = Some (bound, comm))).
 
-Definition know_hist (ms : list fake_map_ty) (uid : w64) (hist : list lat_val_ty) :=
-  (∀ ep lat, hist !! ep = Some lat → know_hist_val ms uid ep lat).
+Definition know_hist (ms : list map_ty) (uid : w64) (hist : list lat_val_ty) :=
+  (∀ (ep : w64) lat, hist !! uint.nat ep = Some lat → know_hist_val ms uid ep lat).
 
 (* hist_msv says that for every latest val in the hist,
 we can derive an msv for it. *)
-Lemma hist_msv ms uid hist ep m lat :
+Lemma hist_msv ms uid hist (ep : w64) m lat :
   adtr_inv' ms →
   know_hist ms uid hist →
-  hist !! ep = Some lat →
-  ms !! ep = Some m →
+  hist !! uint.nat ep = Some lat →
+  ms !! uint.nat ep = Some m →
   msv m uid lat.
 Proof.
   intros Hadtr Hhist Hlook_hist Hlook_m.
-  specialize (Hhist _ _ Hlook_hist) as (vals&?&?&Hhist&Hbound).
+  specialize (Hhist _ _ Hlook_hist) as (vals&?&?&?&Hhist&Hbound).
   exists vals. split_and?; [done..|]. split; [|destruct Hbound as [Hbound|Hbound]].
-  - intros ?? Hlook_ver.
+  - split; [done|]. intros ?? Hlook_ver.
     specialize (Hhist _ _ Hlook_ver) as (?&?&?&?Hlook_prior&?).
     opose proof ((proj1 Hadtr) _ _ _ _ Hlook_prior Hlook_m _); [lia|].
     by eapply lookup_weaken.
@@ -197,7 +198,7 @@ Proof.
     opose proof ((proj1 Hadtr) _ _ _ _ Hlook_m Hlook_bound _); [lia|].
     by eapply lookup_weaken_None.
   - destruct Hbound as (?&?&?&?&Hlook_bound&?).
-    destruct (decide $ is_Some $ m !! (uid, length vals)) as [[? Hlook_mkey]|]; last first.
+    destruct (decide $ is_Some $ m !! (uid, W64 (length vals))) as [[? Hlook_mkey]|]; last first.
     { by eapply eq_None_not_Some. }
     opose proof ((proj1 Hadtr) _ _ _ _ Hlook_m Hlook_bound _); [lia|].
     opose proof (lookup_weaken _ _ _ _ Hlook_mkey _); [done|]. simplify_eq/=.
@@ -211,21 +212,17 @@ Section proper_adtr_inv.
 Definition lower_adtr (m : map_adtr_ty) : merkle_map_ty :=
   (λ v, MapValPre.encodesF (MapValPre.mk v.1 v.2)) <$> m.
 
-(* lookup_weaken_None and lookup_weaken are useful with this. *)
 Definition maps_mono (ms : list merkle_map_ty) :=
-  ∀ i j mi mj,
+  ∀ (i j : nat) mi mj,
   ms !! i = Some mi →
   ms !! j = Some mj →
   i ≤ j →
   mi ⊆ mj.
 
-(* note: auditor allows entry to be added after expected.
-but originating client ensures that doesn't happen. *)
 Definition maps_epoch_ok (ms : list map_adtr_ty) :=
-  ∀ ep m_ep k ep' comm,
+  ∀ (ep : nat) m_ep k ep' comm,
   ms !! ep = Some m_ep →
   m_ep !! k = Some (ep', comm) →
-  (* can't have new entries in an old epoch. *)
   uint.nat ep' ≤ ep.
 
 Definition adtr_inv ms := maps_mono (lower_adtr <$> ms) ∧ maps_epoch_ok ms.
